q2

A1/Q2.dfy
@@ -1,6 +1,6 @@
 predicate sorted(a:array<int>, min:int, max:int)
 requires a != null;
-requires 0 <= min <= max <= a.Length;
+requires 0 < min <= max < a.Length;
 reads a;
 {
     forall j, k :: min <= j < k < max ==> a[j] <= a[k]
@@ -9,65 +9,40 @@ reads a;
 // Find maximum element in the array between left and right
 function method findMax (a: array<int>, left: int, right: int): int
     requires a != null && a.Length > 0;
-    requires 0 < left <= right < a.Length;
+    requires 0 < left < right < a.Length;
     reads a;
     decreases right - left;
+    ensures  0 < left < right < a.Length;
 {
-    if (left == right) then a[left] else 
+    if (left < right) then right else 
         if (a[left] < a[right]) then findMax(a, left + 1, right) else findMax(a, left, right - 1)
 }
-
 
 // Find minimum element in the array between left and right
 function method findMin (a: array<int>, left: int, right: int): int
     requires a != null && a.Length > 0;
-    requires 0 < left <= right < a.Length;
+    requires 0 < left < right < a.Length;
     reads a;
     decreases right - left;
+    ensures  0 < left < right < a.Length;
 {
-    if (left == right) then a[left] else 
+    if (left < right) then left else 
         if (a[left] < a[right]) then findMin(a, left, right - 1) else findMin(a, left + 1, right)
 }
-
-// Find the bigger one, a[left] or a[right]
-function max (a: array<int>, left: int, right: int): int
-    requires a != null && a.Length > 0;
-    requires 0 < left <= right < a.Length;
-    reads a;
-{
-    if (a[left] > a[right]) then a[left] else a[right]
-}
-
-// Find the smaller one, a[left] or a[right]
-function min (a: array<int>, left: int, right: int): int
-    requires a != null && a.Length > 0;
-    requires 0 < left <= right < a.Length;
-    reads a;
-{
-    if (a[left] > a[right]) then a[right] else a[left]
-}
-
-// method testFindMin(a: array <int>, left: int, right: int) returns (index: int)
-//     requires a != null;
-//     requires a.Length > 0;
-//     requires 1 <= left <= right <= a.Length - 1;
-//     requires forall j:: left <= j <= right ==> a[j] >= a[0];
-//     ensures forall j:: left <= j <= right ==> a[j] >= a[index];
-// {
-//     index := findMin(a, left, right);
-// }
 
 method stoogeSort(a: array <int>, left: int, right: int) 
     requires a != null;
     requires a.Length > 0;
-    requires 1 <= left <= right <= a.Length - 1;
+    requires 0 < left < right < a.Length;
+    requires 0 < findMin(a, left, right) < a.Length;
+    requires 0 < findMax(a, left, right) < a.Length;
     modifies a;
-    //ensures sorted(a, left, right);
+    ensures sorted(a, left, right);
     ensures forall i :: (0 <= i < left || right < i < a.Length) ==> a[i] == old(a[i]);
-    ensures a[left] == findMin(a, left, right);
-    //ensures a[right] == findMax(a,left,right);
-    //ensures findMin(a, left, right) == old(findMin(a, left, right));
-    //ensures findMax(a, left, right) == old(max(a, left, right));
+    ensures a[left] == a[findMin(a, left, right)];
+    ensures a[right] == a[findMax(a, left, right)];
+    ensures findMin(a, left, right) == old(findMin(a, left, right));
+    ensures findMax(a, left, right) == old(findMax(a, left, right));
 
     decreases right - left;
 {
@@ -84,6 +59,24 @@ method stoogeSort(a: array <int>, left: int, right: int)
     stoogeSort(a, left, right - k); // First two-thirds
     stoogeSort(a, left + k, right); // Last two-thirds
     stoogeSort(a, left, right - k); // First two-thirds again
+}
+
+// Find the bigger one, a[left] or a[right]
+function method max (a: array<int>, left: int, right: int): int
+    requires a != null && a.Length > 0;
+    requires 0 < left <= right < a.Length;
+    reads a;
+{
+    if (a[left] > a[right]) then left else right
+}
+
+// Find the smaller one, a[left] or a[right]
+function method min (a: array<int>, left: int, right: int): int
+    requires a != null && a.Length > 0;
+    requires 0 < left <= right < a.Length;
+    reads a;
+{
+    if (a[left] > a[right]) then right else left
 }
 /*
 Note from professor in 2013 year
